more CAD

CAD.dfy
@@ -1,11 +1,11 @@
-// RUN: /rlimit:500000
+// RUN: /compile:0 /rlimit:500000
 
 datatype Expr =
     | Empty
     | Unit
     | Translate(r: real, e: Expr)
     | Scale(r: real, e: Expr)
-    /*| Home(r: real, e: Expr)*/
+    /*| Home(r: real, e: Expr)*/  // I don't want to deal with bbox for now
     | Intersect(e1: Expr, e2: Expr)
     | Union(e1: Expr, e2: Expr)
     | Difference(e1: Expr, e2: Expr)
@@ -32,15 +32,32 @@ function ClosedInterval(a: real, b: real): iset<real>
 
 function DenoteTranslate(r: real, S: iset<real>): iset<real>
 {
-    iset x | x in S :: r + x
+    iset x {:nowarn} | x - r in S
 }
 
 
 function DenoteScale(r: real, S: iset<real>): iset<real>
 {
-    iset x | x in S :: r * x
+    if r == 0.0 then iset{}
+    else iset x {:nowarn} | x / r in S
 }
 
+
+// The following example shows that the semantics of difference cannot
+// be A - B, but must be A - cl(B)
+
+function HalfOpenInterval(): iset<real>
+{
+    OpenInterval(-0.5, 0.5) - OpenInterval(0.0, 0.5)
+}
+
+// Construct the singleton set containing 0.0
+lemma Bad()
+    ensures forall x | x in HalfOpenInterval() && x in DenoteScale(-1.0, HalfOpenInterval()) :: x == 0.0
+{}
+
+
+// ⦇e⦈
 function OpenDenote(e: Expr): iset<real>
 {
     match e
@@ -50,7 +67,7 @@ function OpenDenote(e: Expr): iset<real>
         case Scale(r,e) => DenoteScale(r, OpenDenote(e))
         case Intersect(e1,e2) => OpenDenote(e1) * OpenDenote(e2)
         case Union(e1,e2) => OpenDenote(e1) + OpenDenote(e2)
-        case Difference(e1,e2) => OpenDenote(e1) - OpenDenote(e2)
+        case Difference(e1,e2) => OpenDenote(e1) - Closure(OpenDenote(e2))
 }
 
 function abs(r: real): real
@@ -78,7 +95,7 @@ function max(a: real, b: real): real
 
 predicate InBall(center: real, r: real, x: real)
 {
-    abs(center - x) <= r
+    abs(center - x) < r
 }
 
 function Ball(center: real, r: real): iset<real>
@@ -86,16 +103,17 @@ function Ball(center: real, r: real): iset<real>
     iset x | InBall(center, r, x)
 }
 
-predicate InClosure(S: iset<real>, x: real)
+predicate InClosure(x: real, S: iset<real>)
 {
-    forall eps | eps > 0.0 :: Ball(x, eps) * S != iset{}
+    forall eps | eps > 0.0 :: !(Ball(x, eps) !! S)
 }
 
 function Closure(S: iset<real>): iset<real>
 {
-    iset x | InClosure(S, x)
+    iset x | InClosure(x, S)
 }
 
+// ⟦e⟧
 function Denote(e: Expr): iset<real>
 {
     Closure(OpenDenote(e))
@@ -116,119 +134,46 @@ lemma ClosureOpenInterval(a: real, b: real)
         if x < a {
             var eps := (a - x) / 2.0;
             var y :| y in Ball(x, eps) * OpenInterval(a, b);
-            assert x in ClosedInterval(a, b);
         } else if x > b {
             var eps := (x - b) / 2.0;
             var y :| y in Ball(x, eps) * OpenInterval(a, b);
-            assert x in ClosedInterval(a, b);
-        } else {
-            assert x in ClosedInterval(a, b);
         }
     }
 
     forall x | x in ClosedInterval(a, b)
         ensures x in Closure(OpenInterval(a, b))
     {
-        if x == a {
-            forall eps | eps > 0.0
-                ensures Ball(a, eps) * OpenInterval(a, b) != iset{}
-            {
-                var d := min(eps, (b - a) / 2.0);
+        forall eps | eps > 0.0
+            ensures Ball(x, eps) * OpenInterval(a, b) != iset{}
+        {
+            if x == a {
+                var d := min(eps, b - a) / 2.0;
+                assert x + d in Ball(a, eps);
                 ISetNonEmpty(x + d, Ball(a, eps) * OpenInterval(a, b));
-            }
-
-            assert x in Closure(OpenInterval(a, b));
-        } else if x == b {
-            forall eps | eps > 0.0
-                ensures Ball(b, eps) * OpenInterval(a, b) != iset{}
-            {
-                var d := min(eps, (b - a) / 2.0);
+            } else if x == b {
+                var d := min(eps, b - a) / 2.0;
                 ISetNonEmpty(x - d, Ball(b, eps) * OpenInterval(a, b));
-            }
-
-            assert x in Closure(OpenInterval(a, b));
-        } else {
-            forall eps | eps >= 0.0
-                ensures Ball(x, eps) * OpenInterval(a, b) != iset{}
-            {
+            } else {
                 ISetNonEmpty(x, Ball(x, eps) * OpenInterval(a, b));
             }
-
-            assert x in Closure(OpenInterval(a, b));
         }
     }
 }
 
-lemma TranslateOpenInterval(r: real, a: real, b: real)
-    ensures DenoteTranslate(r, OpenInterval(a, b)) == OpenInterval(r + a, r + b)
-{
-    forall x: real
-        ensures x in DenoteTranslate(r, OpenInterval(a, b)) <==> x in OpenInterval(r + a, r + b)
-    {
-        calc {
-            x in DenoteTranslate(r, OpenInterval(a, b));
-            <==> x in (iset y | y in OpenInterval(a, b) :: r + y);
-            <==> {
-                if r + a < x < r + b {
-                    assert x - r in OpenInterval(a, b);
-                }
-            } r + a < x < r + b;
-            <==> x in OpenInterval(r + a, r + b);
-        }
-
-    }
-}
-
-lemma ScaleOpenInterval(r: real, a: real, b: real)
-    requires r > 0.0
-    ensures DenoteScale(r, OpenInterval(a, b)) == OpenInterval(r * a, r * b)
-{
-    forall x: real
-        ensures x in DenoteScale(r, OpenInterval(a, b)) <==> x in OpenInterval(r * a, r * b)
-    {
-        calc {
-            x in DenoteScale(r, OpenInterval(a, b));
-            <==> x in (iset y | y in OpenInterval(a, b) :: r * y);
-            <==> {
-                if r * a < x < r * b {
-                    var y := x / r;
-                    assert y in OpenInterval(a, b);
-                    assert r * y == x;
-                }
-            } r * a < x < r * b;
-            <==> x in OpenInterval(r * a, r * b);
-        }
-
-    }
-}
+lemma ClosureUnion(A: iset<real>, B: iset<real>)
+    ensures Closure(A + B) == Closure(A) + Closure(B)
+{ }
 
 lemma CloseAdjacentOpenIntervals(a: real, b: real, c: real)
     requires a <= b <= c
     ensures Closure(OpenInterval(a, b) + OpenInterval(b, c)) == Closure(OpenInterval(a, c))
 {
     if a == b || b == c { return; }
+
+    ClosureUnion(OpenInterval(a,b), OpenInterval(b,c));
     ClosureOpenInterval(a, c);
-    var S := OpenInterval(a, b) + OpenInterval(b, c);
-    forall x | x in ClosedInterval(a, c)
-        ensures x in Closure(S);
-    {
-        forall eps | eps > 0.0
-            ensures Ball(x, eps) * S != iset{}
-        {
-            if x == a {
-                ISetNonEmpty(x + min(eps, (b - a)) / 2.0, Ball(x, eps) * S);
-                assert Ball(x, eps) * S != iset{};
-            } else if x == b {
-                ISetNonEmpty(x - min(eps, (b - a)) / 2.0, Ball(x, eps) * S);
-                assert Ball(x, eps) * S != iset{};
-            } else if x == c {
-                ISetNonEmpty(x - min(eps, (c - b)) / 2.0, Ball(x, eps) * S);
-                assert Ball(x, eps) * S != iset{};
-            } else {
-                ISetNonEmpty(x, Ball(x, eps) * S);
-            }
-        }
-    }
+    ClosureOpenInterval(a, b);
+    ClosureOpenInterval(b, c);
 }
 
 lemma UnionUnitTest()
@@ -236,21 +181,182 @@ lemma UnionUnitTest()
 {
     calc {
         Denote(Union(Unit, Translate(1.0, Unit)));
-        == Closure(OpenDenote(Union(Unit, Translate(1.0, Unit)))); 
-        == {
-            calc {
-                OpenDenote(Union(Unit, Translate(1.0, Unit)));
-                == OpenInterval(0.0, 1.0) + DenoteTranslate(1.0, OpenInterval(0.0, 1.0));
-                == { TranslateOpenInterval(1.0, 0.0, 1.0); }
-                   OpenInterval(0.0, 1.0) + OpenInterval(1.0, 2.0);
-            }
-        }
-        Closure(OpenInterval(0.0, 1.0) + OpenInterval(1.0, 2.0));
+        == Closure(OpenDenote(Union(Unit, Translate(1.0, Unit))));
+        == Closure(OpenInterval(0.0, 1.0) + DenoteTranslate(1.0, OpenInterval(0.0, 1.0)));
+        == Closure(OpenInterval(0.0, 1.0) + OpenInterval(1.0, 2.0));
         == { CloseAdjacentOpenIntervals(0.0, 1.0, 2.0); }
            Closure(OpenInterval(0.0, 2.0));
-        == { ScaleOpenInterval(2.0, 0.0, 1.0); }
-           Closure(DenoteScale(2.0, OpenInterval(0.0, 1.0)));
+        == Closure(DenoteScale(2.0, OpenInterval(0.0, 1.0)));
         == Closure(OpenDenote(Scale(2.0, Unit)));
         == Denote(Scale(2.0, Unit));
+    }
+}
+
+predicate Open(S: iset<real>)
+{
+    forall x | x in S :: exists eps | eps > 0.0 :: Ball(x, eps) <= S
+}
+
+lemma OpenIntervalOpen(a: real, b: real)
+    requires a < b
+    ensures Open(OpenInterval(a, b))
+{
+    var S := OpenInterval(a, b);
+    forall x | x in S
+        ensures exists eps | eps > 0.0 :: Ball(x, eps) <= S
+    {
+        var eps := min((x - a) / 2.0, (b - x) / 2.0);
+        assert Ball(x, eps) <= S;
+    }
+}
+
+lemma DenoteTranslateOpen(r: real, S: iset<real>)
+    requires Open(S)
+    ensures Open(DenoteTranslate(r, S))
+{
+    var S' := DenoteTranslate(r, S);
+    forall x | x in S'
+        ensures exists eps | eps > 0.0 :: Ball(x, eps) <= S'
+    {
+        var y := x - r;
+        assert y in S;
+        var eps :| eps > 0.0 && Ball(y, eps) <= S;
+
+        assert Ball(x, eps) <= S';
+    }
+}
+
+lemma DenoteScaleOpen(r: real, S: iset<real>)
+    requires Open(S)
+    ensures Open(DenoteScale(r, S))
+{
+    if r == 0.0 { return; }
+    var S' := DenoteScale(r, S);
+    forall x | x in S'
+        ensures exists eps | eps > 0.0 :: Ball(x, eps) <= S'
+    {
+        var y := x / r;
+        assert y in S;
+        var eps :| eps > 0.0 && Ball(y, eps) <= S;
+
+        assert Ball(x, abs(r) * eps) <= S';
+    }
+}
+
+function R(): iset<real>
+{
+    iset x {:nowarn} | true
+}
+
+predicate Closed(S: iset<real>)
+{
+    S == Closure(S)
+}
+
+lemma ClosureIdempotent(S: iset<real>)
+    ensures Closure(Closure(S)) == Closure(S)
+{
+    forall x | x in Closure(Closure(S))
+        ensures x in Closure(S)
+    {
+        forall eps | eps > 0.0
+            ensures !(Ball(x, eps) !! S)
+        {
+            var y :| y in Ball(x, eps / 2.0) && y in Closure(S);
+            var z :| z in Ball(y, eps / 2.0) && z in S;
+        }
+    }
+}
+
+lemma ClosureClosed(S: iset<real>)
+    ensures Closed(Closure(S))
+{
+    ClosureIdempotent(S);
+}
+
+
+lemma DisjointIntersectionEmpty<T>(A: iset<T>, B: iset<T>)
+    requires A * B == iset{}
+    ensures A !! B
+{
+    forall a, b | a in A && b in B
+        ensures a != b
+    {
+        if a == b {
+            assert a in A * B;
+            ISetNonEmpty(a, A * B);
+        }
+    }
+}
+
+lemma ComplementClosedOpen(S: iset<real>)
+    requires Closed(S)
+    ensures Open(R() - S)
+{
+    var D := R() - S;
+    forall x | x in D
+        ensures exists eps | eps > 0.0 :: Ball(x, eps) <= D
+    {
+        assert x !in Closure(S);
+        var eps :| eps > 0.0 && Ball(x, eps) * S == iset{};
+        DisjointIntersectionEmpty(Ball(x, eps), S);
+        assert Ball(x, eps) <= D;
+    }
+}
+
+lemma IntersectOpen(S1: iset<real>, S2: iset<real>)
+    requires Open(S1) && Open(S2)
+    ensures Open(S1 * S2)
+{}
+
+lemma DifferenceOpen(S1: iset<real>, S2: iset<real>)
+    requires Open(S1)
+    ensures Open(S1 - Closure(S2))
+{
+    assert S1 - Closure(S2) == S1 * (R() - Closure(S2));
+    ClosureClosed(S2);
+    ComplementClosedOpen(Closure(S2));
+    IntersectOpen(S1, R() - Closure(S2));
+}
+
+
+lemma OpenDenoteOpen(e: Expr)
+    ensures Open(OpenDenote(e))
+{
+    match e {
+        case Empty => {}
+        case Unit => { OpenIntervalOpen(0.0, 1.0); }
+        case Translate(r, e) => { DenoteTranslateOpen(r, OpenDenote(e)); }
+        case Scale(r, e) => { DenoteScaleOpen(r, OpenDenote(e)); }
+        case Intersect(e1, e2) => {}
+        case Union(e1, e2) => {}
+        case Difference(e1, e2) => { DifferenceOpen(OpenDenote(e1), OpenDenote(e2)); }
+    }
+}
+
+predicate NoIsolatedPoints(S: iset<real>)
+{
+    forall x, eps | x in S && eps > 0.0 :: !((Ball(x, eps) - iset{x}) !! S)
+}
+
+lemma DenoteNoIsolatedPoints(e: Expr)
+    ensures NoIsolatedPoints(Denote(e))
+{
+    forall x, eps | x in Denote(e) && eps > 0.0
+        ensures exists z :: z in Ball(x, eps) && z != x && z in Denote(e)
+    {
+        assert !(OpenDenote(e) !! Ball(x, eps / 2.0));
+        var y :| y in OpenDenote(e) && y in Ball(x, eps / 2.0);
+        if x == y {
+            OpenDenoteOpen(e);
+            var eps' :| eps' > 0.0 && Ball(y, eps') <= OpenDenote(e);
+            var eps'' := min(eps, eps') / 2.0;
+            var z := x + eps'';
+            assert z in Ball(y, eps');
+            assert z in Denote(e);
+        } else {
+            assert y in Denote(e);
+        }
+
     }
 }
